theories/designs/utp_des_core.thy
@@ -379,15 +379,15 @@ theorem design_composition_wp:
   assumes
     "ok \<sharp> p1" "ok \<sharp> p2"
     "$ok \<sharp> Q1" "$ok\<acute> \<sharp> Q1" "$ok \<sharp> Q2" "$ok\<acute> \<sharp> Q2"
-  shows "((\<lceil>p1\<rceil>\<^sub>< \<turnstile> Q1) ;; (\<lceil>p2\<rceil>\<^sub>< \<turnstile> Q2)) = ((\<lceil>p1 \<and> Q1 wp p2\<rceil>\<^sub><) \<turnstile> (Q1 ;; Q2))"
+  shows "((\<lceil>p1\<rceil>\<^sub>< \<turnstile> Q1) ;; (\<lceil>p2\<rceil>\<^sub>< \<turnstile> Q2)) = ((\<lceil>p1 \<and> Q1 wlp p2\<rceil>\<^sub><) \<turnstile> (Q1 ;; Q2))"
   using assms by (rel_blast)
 
 theorem rdesign_composition_wp:
-  "((\<lceil>p1\<rceil>\<^sub>< \<turnstile>\<^sub>r Q1) ;; (\<lceil>p2\<rceil>\<^sub>< \<turnstile>\<^sub>r Q2)) = ((\<lceil>p1 \<and> Q1 wp p2\<rceil>\<^sub><) \<turnstile>\<^sub>r (Q1 ;; Q2))"
+  "((\<lceil>p1\<rceil>\<^sub>< \<turnstile>\<^sub>r Q1) ;; (\<lceil>p2\<rceil>\<^sub>< \<turnstile>\<^sub>r Q2)) = ((\<lceil>p1 \<and> Q1 wlp p2\<rceil>\<^sub><) \<turnstile>\<^sub>r (Q1 ;; Q2))"
   by (rel_blast)
 
 theorem ndesign_composition_wp [ndes_simp]:
-  "((p1 \<turnstile>\<^sub>n Q1) ;; (p2 \<turnstile>\<^sub>n Q2)) = ((p1 \<and> Q1 wp p2) \<turnstile>\<^sub>n (Q1 ;; Q2))"
+  "((p1 \<turnstile>\<^sub>n Q1) ;; (p2 \<turnstile>\<^sub>n Q2)) = ((p1 \<and> Q1 wlp p2) \<turnstile>\<^sub>n (Q1 ;; Q2))"
   by (rel_blast)
 
 theorem design_true_left_zero: "(true ;; (P \<turnstile> Q)) = true"
